Test/Tactics/FirstOrder.lean
@@ -11,8 +11,6 @@ example : True := by
 
 set_option pp.explicit true in
 set_option trace.auto.buildChecker true in
-set_option trace.auto.mono true in
-set_option trace.auto.mono.printConstInst true in
 example (a b : Prop) : a ∨ b ∨ ¬ a := by
   auto
 
@@ -24,8 +22,6 @@ example (a b : Nat) (f : Nat → Nat)
 set_option trace.auto.tactic true in
 set_option trace.auto.buildChecker true in
 set_option trace.auto.printLemmas true in
-set_option trace.auto.mono.printConstInst true in
-set_option trace.auto.mono true in
 set_option trace.auto.lamReif true in
 example {α β : Type} (a : α) (b : β) (H : b = b) : a = a := by
   auto [H]
@@ -34,7 +30,6 @@ set_option pp.raw true in
 set_option trace.auto.buildChecker true in
 set_option trace.auto.tactic true in
 set_option trace.auto.lamReif true in
-set_option trace.auto.mono.printLemmaInst true in
 example (a : Nat) (f : Nat → Nat) (H : ∀ x, f x = x) :
   f x = f (f (f (f (f (f (f (f (f x)))))))) := by
   auto [H]
